Iterator/Combinators/FilterMap.lean
@@ -24,85 +24,95 @@ section FilterMapMH
 universe u' v' u v
 
 @[ext]
-structure FilterMapMH (α : Type u) {β : Type v} {γ : Type v'}
-    {m : Type w → Type w'} (f : β → IterationT m (Option γ)) where
+structure FilterMapMH (α : Type u) {β : Type v} {γ : Type v'} [Small.{w} γ]
+    {m : Type w → Type w'} {p : Option γ → Prop} (f : β → m (USquash <| Subtype p)) where
   inner : α
 
-def MapMH (α : Type u) {β : Type v} {γ : Type v'} {m : Type w → Type w'} (f : β → IterationT m γ) :=
-  FilterMapMH α (some <$> f ·)
+def MapMH (α : Type u) {β : Type v} {γ : Type v'} {m : Type w → Type w'} [Functor m]
+    [Small.{w} γ] {p : γ → Prop} (f : β → m (USquash <| Subtype p)) :=
+  FilterMapMH α (γ := γ) (p := fun x => ∃ y, x = some y ∧ p y)
+    (fun x => (USquash.deflate ∘ (fun y => ⟨some y.1, y.1, rfl, y.2⟩) ∘ USquash.inflate) <$> f x)
 
-variable {α : Type u} {m : Type w → Type w'} {β : Type v} {γ : Type v'}
-    [Monad m] [Iterator α m β]
-    {f : β → IterationT m (Option γ)}
+variable {α : Type u} {m : Type w → Type w'} {β : Type v} {γ : Type v'} [Small.{w} γ]
+    [Monad m] [Iterator α m β] {p : Option γ → Prop} {f : β → m (USquash <| Subtype p)}
 
-instance [i : ComputableSmall.{w} α] : ComputableSmall.{w} (FilterMapMH α f) :=
-  i.equiv FilterMapMH.mk FilterMapMH.inner rfl rfl
+instance : Small.{w} (FilterMapMH α f) where
+  h := haveI : Small.{w} α := Iterator.state_small m; ⟨{
+    Target := USquash α
+    deflate x := .deflate x.inner
+    inflate x := .mk x.inflate
+    deflate_inflate := by simp
+    inflate_deflate := by simp
+  }⟩
 
-instance [i : ComputableSmall.{w} α] {f : β → IterationT m γ} : ComputableSmall.{w} (MapMH α f) :=
-  instComputableSmallFilterMapMH
+inductive FilterMapMH.PlausibleStep (it : FilterMapMH α f) : (step : IterStep (FilterMapMH α f) γ) → Prop where
+  | yieldNone : ∀ {it' out}, Iterator.plausible_step m it.inner (.yield it'.inner out) → p none → PlausibleStep it (.skip it')
+  | yieldSome : ∀ {it' out out'}, Iterator.plausible_step m it.inner (.yield it'.inner out) → p (some out') → PlausibleStep it (.yield it' out')
+  | skip : ∀ {it'}, Iterator.plausible_step m it.inner (.skip it'.inner) → PlausibleStep it (.skip it')
+  | done : Iterator.plausible_step m it.inner .done → PlausibleStep it .done
 
 instance : Iterator (FilterMapMH α f) m γ where
-  step it :=
-    Iterator.step (m := m) it.inner |>.bindH <| matchStep
-      (fun it' b => IterationT.mapH
-        (match · with
-          | none => .skip ⟨it'⟩
-          | some c => .yield ⟨it'⟩ c) (f b))
-      (fun it' => pure <| .skip ⟨it'⟩)
-      (pure <| .done)
+  state_small := inferInstance
+  value_small := inferInstance
+  plausible_step := FilterMapMH.PlausibleStep
+  step it := do
+    let step ← Iterator.step (m := m) it.inner
+    letI step' := step.inflate (small := _)
+    match step' with
+    | .yield it' out h => do
+      match (← f out).inflate with
+      | ⟨none, h'⟩ => pure <| .deflate <| .skip ⟨it'⟩ (.yieldNone h h')
+      | ⟨some out', h'⟩ => pure <| .deflate <| .yield ⟨it'⟩ out' (.yieldSome h h')
+    | .skip it' h => pure <| .deflate <| .skip ⟨it'⟩ (.skip h)
+    | .done h => pure <| .deflate <| .done (.done h)
 
-instance {f : β → IterationT m γ} : Iterator (MapMH α f) m γ :=
+instance {p : γ → Prop} {f : β → m (USquash <| Subtype p)} :
+    Iterator (MapMH α f) m γ :=
   inferInstanceAs <| Iterator (FilterMapMH α _) m γ
 
 -- TODO: This proof needs to use internals of IterationT instead of relying on successor_yield
 instance [Finite α m] : FinitenessRelation (FilterMapMH α f) m where
-  rel := InvImage (Iterator.successor_of m) FilterMapMH.inner
+  rel := InvImage (Iterator.plausible_successor m) FilterMapMH.inner
   wf := InvImage.wf _ Finite.wf
   subrelation {it it'} h := by
-    simp only [Iterator.step] at h
-    match successor_matchStepH h with
-    | .yield hy h =>
-      simp only [IterationT.mapH, Function.comp_apply] at h
-      obtain ⟨h, hb, a, rfl, h'⟩ := h
-      split at hb
-      · cases hb
-        exact Iterator.successor_of_yield hy
-      · cases hb
-        exact Iterator.successor_of_yield hy
-    | .skip hs h =>
-      cases successor_skip.mp h
-      exact Iterator.successor_of_skip hs
-    | .done hd h =>
-      cases successor_done.mp h
+    simp only [Iterator.plausible_successor, Iterator.plausible_step] at h
+    obtain ⟨step, h, h'⟩ := h
+    cases h'
+    case yieldNone it' out h' h'' =>
+      cases h
+      exact Iterator.successor_of_yield h'
+    case yieldSome it' out h' h'' =>
+      cases h
+      exact Iterator.successor_of_yield h'
+    case skip it' h' =>
+      cases h
+      exact Iterator.successor_of_skip h'
+    case done h' =>
+      cases h
 
-instance {f : β → IterationT m γ} [Finite α m] : Finite (MapMH α f) m :=
+instance {p : γ → Prop} {f : β → m (USquash <| Subtype p)} [Finite α m] :
+    Finite (MapMH α f) m :=
   inferInstanceAs <| Finite (FilterMapMH α _) m
 
-instance {f : β → IterationT m γ} [Productive α m] : ProductivenessRelation (MapMH α f) m where
-  rel := InvImage (Iterator.skip_successor_of m) FilterMapMH.inner
+instance {p : γ → Prop} {f : β → m (USquash <| Subtype p)} [Productive α m] :
+    ProductivenessRelation (MapMH α f) m where
+  rel := InvImage (Iterator.plausible_skip m) FilterMapMH.inner
   wf := InvImage.wf _ Productive.wf
   subrelation {it it'} h := by
-    simp only [Iterator.step] at h
-    match property_matchStepH h with
-    | .yield hy h =>
-      simp only [IterationT.mapH] at h
-      obtain ⟨c, h, h'⟩ := h
-      split at h
-      · simp [Functor.map] at h'
-      · cases h
-    | .skip hs h =>
-      cases h
-      exact hs
-    | .done hd h =>
-      cases h
+    simp only [Iterator.plausible_skip, Iterator.plausible_step] at h
+    cases h
+    case yieldNone it' out h h' =>
+      simp at h
+    case skip it' h =>
+      exact h
 
 @[always_inline, inline]
-def Iterator.filterMapMH [Monad m] [Iterator α m β] (f : β → IterationT m (Option γ)) (it : α) :
+def Iterator.filterMapMH [Monad m] [Iterator α m β] (f : β → m (USquash <| Subtype p)) (it : α) :
     FilterMapMH α (m := m) f :=
   ⟨it⟩
 
 @[always_inline, inline]
-def Iterator.mapMH [Monad m] [Iterator α m β] (f : β → IterationT m γ) (it : α) :
+def Iterator.mapMH [Monad m] [Iterator α m β] {p : γ → Prop} (f : β → m (USquash <| Subtype p)) (it : α) :
     MapMH α (m := m) (f ·) :=
   ⟨it⟩
 
@@ -130,9 +140,10 @@ it.filterMapMH     ---a'-----c'-------⊥
 This combinator incurs an additional O(1) cost with each output of `it` in addition to the cost of the monadic effects.
 -/
 @[inline]
-def Iter.filterMapMH [Monad m] {_ : Iterator α m β} {_ : ComputableSmall.{w} α} (f : β → CodensityT m (Option γ))
+def Iter.filterMapMH [Monad m] {_ : Iterator α m β} (f : β → m (USquash <| Option γ))
     (it : Iter (α := α) m β) :=
-  ((toIter m <| Iterator.filterMapMH (m := m) (monadLift <| f ·) it.inner) : Iter m γ)
+  ((toIter m <| Iterator.filterMapMH (m := m) (p := fun _ => True)
+    ((USquash.deflate ∘ (⟨·, True.intro⟩) ∘ USquash.inflate) <$> f ·) it.inner) : Iter m γ)
 
 /--
 Given an iterator `it`, a monadic mapping function `f` and a monad transformation `mf`,
@@ -160,8 +171,9 @@ _TODO_: prove `Productive`. This requires us to wrap the FilterMapMH into a new 
 This combinator incurs an additional O(1) cost with each output of `it` in addition to the cost of the monadic effects.
 -/
 @[inline]
-def Iter.mapMH [Monad m] {_ : Iterator α m β} {_ : ComputableSmall.{w} α} (f : β → CodensityT m γ) (it : Iter (α := α) m β) :=
-  (toIter m <| Iterator.mapMH (m := m) (monadLift <| f ·) it.inner : Iter m γ)
+def Iter.mapMH [Monad m] {_ : Iterator α m β} (f : β → m (USquash γ)) (it : Iter (α := α) m β) :=
+  (toIter m <| Iterator.mapMH (m := m) (p := fun _ => True)
+    ((USquash.deflate ∘ (⟨·, True.intro⟩) ∘ USquash.inflate) <$> f ·) it.inner : Iter m γ)
 
 /--
 Given an iterator `it`, a monadic predicate `p` and a monad transformation `mf`,
@@ -187,8 +199,10 @@ it.filterMH        ---a-----c-------⊥
 This combinator incurs an additional O(1) cost with each output of `it` in addition to the cost of the monadic effects.
 -/
 @[inline]
-def Iter.filterMH [Monad m] {_ : Iterator α m β} {_ : ComputableSmall.{w} α} (f : β → CodensityT m Bool) (it : Iter (α := α) m β) :=
-  it.filterMapMH (fun b => (f b).mapH (if · then some b else none))
+def Iter.filterMH [Monad m] {_ : Iterator α m β} (f : β → m (USquash Bool)) (it : Iter (α := α) m β) :=
+  haveI : Small.{w} β := Iterator.value_small α m
+  it.filterMapMH
+    (fun b => (USquash.deflate ∘ (if · = true then some b else none) ∘ USquash.inflate) <$> (f b))
 
 end FilterMapMH
 
@@ -197,15 +211,15 @@ section FilterMapH
 universe u' v' u v
 
 variable {α : Type u} {β : Type v} {m : Type w → Type w'} [Monad m] [Iterator α m β]
-    {γ : Type v'} {f : β → Option γ}
+    {γ : Type v'} {f : β → Option γ} [Small.{w} γ]
 
 @[inline]
-def Iter.filterMapH [Monad m] {_ : Iterator α m β} {_ : ComputableSmall.{w} α} (f : β → Option γ) (it : Iter (α := α) m β) :=
-  (it.filterMapMH (pure ∘ f) : Iter m γ)
+def Iter.filterMapH (f : β → Option γ) (it : Iter (α := α) m β) :=
+  (it.filterMapMH (pure ∘ USquash.deflate ∘ f) : Iter m γ)
 
 @[inline]
-def Iter.mapH [Monad m] {_ : Iterator α m β} {_ : ComputableSmall.{w} α} (f : β → γ) (it : Iter (α := α) m β) :=
-  (it.mapMH (pure ∘ f) : Iter m γ)
+def Iter.mapH (f : β → γ) (it : Iter (α := α) m β) :=
+  (it.mapMH (pure ∘ USquash.deflate ∘ f) : Iter m γ)
 
 end FilterMapH
 
@@ -213,37 +227,36 @@ section FilterMap
 
 variable {m : Type w → Type w'} {α : Type u} {β : Type v} {γ : Type w} {f : β → Option γ}
 
--- Potential other formulation of iterators: Each iterator type comes with equivalences for all types of the current level.
--- Then the following operations could be stated in higher generality, not requiring y : Type w.
-
 @[inline]
-def Iter.filterMap {_ : Iterator α m β} {_ : ComputableSmall.{w} α} [Monad m] (f : β → Option γ) (it : Iter (α := α) m β) :=
+def Iter.filterMap {_ : Iterator α m β} [Monad m] (f : β → Option γ) (it : Iter (α := α) m β) :=
   (it.filterMapH f : Iter m γ)
 
 @[inline]
-def Iter.map {_ : Iterator α m β} {_ : ComputableSmall.{w} α} [Monad m] (f : β → γ) (it : Iter (α := α) m β) :=
+def Iter.map {_ : Iterator α m β} [Monad m] (f : β → γ) (it : Iter (α := α) m β) :=
   (it.mapH f : Iter m γ)
 
 @[inline]
-def Iter.filter {_ : Iterator α m β} {_ : ComputableSmall.{w} α} [Monad m] (f : β → Bool) (it : Iter (α := α) m β) :=
+def Iter.filter {_ : Iterator α m β} [Monad m] (f : β → Bool) (it : Iter (α := α) m β) :=
+  haveI : Small.{w} β := Iterator.value_small α m
   (it.filterMapH (fun b => if f b then some b else none) : Iter m β)
 
 end FilterMap
 
 section FilterMapM
 
-variable {m : Type w → Type w'} {α : Type u} {β : Type v} {γ : Type w} {f : β → Option γ}
+variable {m : Type w → Type w'} {α : Type w} {β : Type v} {γ : Type w} {f : β → Option γ}
 
 @[inline]
-def Iter.filterMapM {_ : Iterator α m β} {_ : ComputableSmall.{w} α} [Monad m] (f : β → m (Option γ)) (it : Iter (α := α) m β) :=
-  (it.filterMapMH (monadLift ∘ f) : Iter m γ)
+def Iter.filterMapM {_ : Iterator α m β} [Monad m] (f : β → m (Option γ)) (it : Iter (α := α) m β) :=
+  (it.filterMapMH (USquash.deflate <$> f ·) : Iter m γ)
 
 @[inline]
-def Iter.mapM {_ : Iterator α m β} {_ : ComputableSmall.{w} α} [Monad m] (f : β → m γ) (it : Iter (α := α) m β) :=
+def Iter.mapM {_ : Iterator α m β} [Monad m] (f : β → m γ) (it : Iter (α := α) m β) :=
   (it.filterMapM (fun b => some <$> f b) : Iter m γ)
 
 @[inline]
-def Iter.filterM {_ : Iterator α m β} {_ : ComputableSmall.{w} α} [Monad m] (f : β → m (ULift Bool)) (it : Iter (α := α) m β) :=
-  it.filterMapMH (fun b => CodensityT.eval (f b) |>.mapH (if ·.down then some b else none))
+def Iter.filterM {_ : Iterator α m β} [Monad m] (f : β → m (USquash Bool)) (it : Iter (α := α) m β) :=
+  haveI : Small.{w} β := Iterator.value_small α m
+  (it.filterMapMH (fun b => (USquash.deflate ∘ (if · = true then some b else none) ∘ USquash.inflate) <$> f b) : Iter m β)
 
 end FilterMapM
