Iterator/Consumers.lean
@@ -9,12 +9,11 @@ import Iterator.Wrapper
 @[specialize]
 def Iter.forIn {m : Type w → Type w'} {n : Type w → Type w''} [Monad m] [Monad n] [MonadLiftT m n]
     {α : Type u} {β : Type v} {γ : Type w}
-    {_ : Iterator α m β} [Finite α m] {_ : ComputableSmall.{w} α} [ComputableSmall.{w} β]
+    {_ : Iterator α m β} [Finite α m]
     (it : Iter (α := α) m β) (init : γ) (f : β → γ → n (ForInStep γ)) : n γ := do
-  let x : n it.LiftedStep := it.stepH.mapH (·.lift) |>.run
-  match ← x with
-  | .yield it' b _ =>
-    match ← f (ComputableSmall.down b) init with
+  match (← it.stepH).inflate with
+  | .yield it' out _ =>
+    match ← f out init with
     | .yield c => it'.forIn c f
     | .done c => return c
   | .skip it' _ => it'.forIn init f
@@ -28,11 +27,10 @@ instance {m : Type w → Type w'} {n : Type w → Type w''} [Monad m] [Monad n] 
 
 @[specialize]
 def Iter.foldM {m : Type w → Type w'} {n : Type w → Type w'} [Monad m] [Monad n] [MonadLiftT m n]
-    {α : Type u} {β : Type v} {γ : Type w} {_ : Iterator α m β} [Finite α m] {_ : ComputableSmall.{w} α} [ComputableSmall.{w} β]
+    {α : Type u} {β : Type v} {γ : Type w} {_ : Iterator α m β} [Finite α m]
     (f : γ → β → n γ) (init : γ) (it : Iter (α := α) m β) : n γ := do
-  let step : n it.LiftedStep := it.stepH.mapH (·.lift) |>.run
-  match ← step with
-  | .yield it' b _ => it'.foldM f (← f init (ComputableSmall.down b))
+  match (← it.stepH).inflate with
+  | .yield it' b _ => it'.foldM f (← f init b)
   | .skip it' _ => it'.foldM f init
   | .done _ => return init
 termination_by it.terminationByFinite
@@ -43,10 +41,10 @@ def Iter.count {α : Type u} {β : Type v} {_ : Iterator α Id β} [Finite α Id
   go it 0
 where
   go [Finite α Id] it acc :=
-    it.stepH _ (match · with
-      | .yield it' _ _ => go it' (acc + 1)
-      | .skip it' _ => go it' acc
-      | .done _ => return acc)
+    match it.stepH.inflate with
+    | .yield it' _ _ => go it' (acc + 1)
+    | .skip it' _ => go it' acc
+    | .done _ => acc
   termination_by it.terminationByFinite
 
 @[specialize]
@@ -55,29 +53,29 @@ def Iter.countM {m : Type → Type w'} [Monad m] {α : Type u} {β : Type v} {_ 
   go it 0
 where
   go [Finite α m] it acc := do
-    it.stepH _ (match · with
+    match (← it.stepH).inflate with
       | .yield it' _ _ => go it' (acc + 1)
       | .skip it' _ => go it' acc
-      | .done _ => return acc)
+      | .done _ => return acc
   termination_by it.terminationByFinite
 
-@[inline]
-def Iter.toArrayH {α : Type u} {m : Type w → Type w'} [Monad m] {β : Type v}
-    {_ : Iterator α m β} [Finite α m] {_ : ComputableSmall.{w} α} [ComputableUnivLE.{v, w}] (it : Iter (α := α) m β) : CodensityT m (Array β) :=
-  (CodensityT.eval <| go it #[]).mapH ComputableSmall.down
-where
-  @[specialize]
-  go [Monad m] [Finite α m] it a : m (ComputableSmall.Lift.{w} (Array β)) := do
-    let step ← it.stepH.mapH (·.lift) |>.run
-    match step with
-      | .yield it' b _ => go it' (a.push <| ComputableSmall.down b)
-      | .skip it' _ => go it' a
-      | .done _ => return ComputableSmall.up a
-  termination_by it.terminationByFinite
+-- @[inline]
+-- def Iter.toArrayH {α : Type u} {m : Type w → Type w'} [Monad m] {β : Type v}
+--     {_ : Iterator α m β} [Finite α m] (it : Iter (α := α) m β) : m (Array β) :=
+--   (CodensityT.eval <| go it #[]).mapH ComputableSmall.down
+-- where
+--   @[specialize]
+--   go [Monad m] [Finite α m] it a : m (ComputableSmall.Lift.{w} (Array β)) := do
+--     let step ← it.stepH.mapH (·.lift) |>.run
+--     match step with
+--       | .yield it' b _ => go it' (a.push <| ComputableSmall.down b)
+--       | .skip it' _ => go it' a
+--       | .done _ => return ComputableSmall.up a
+--   termination_by it.terminationByFinite
 
 @[inline]
 def Iter.toArray {α : Type u} {m : Type v → Type w} [Monad m] {β : Type v}
-    {_ : Iterator α m β} [Finite α m] {_ : ComputableSmall.{v} α} (it : Iter (α := α) m β) : m (Array β) :=
+    {_ : Iterator α m β} [Finite α m] (it : Iter (α := α) m β) : m (Array β) :=
   go it #[]
 where
   @[specialize]
@@ -90,7 +88,7 @@ where
 
 @[inline]
 def Iter.reverseToList {α : Type u} {m : Type v → Type w} [Monad m] {β : Type v}
-    {_ : Iterator α m β} [Finite α m] {_ : ComputableSmall.{v} α} (it : Iter (α := α) m β) : m (List β) :=
+    {_ : Iterator α m β} [Finite α m] (it : Iter (α := α) m β) : m (List β) :=
   go it []
 where
   @[specialize]
@@ -103,14 +101,14 @@ where
 
 @[inline]
 def Iter.toList {α : Type u} {m : Type v → Type w} [Monad m] {β : Type v}
-    {_ : Iterator α m β} [Finite α m] {_ : ComputableSmall.{v} α} (it : Iter (α := α) m β) : m (List β) :=
+    {_ : Iterator α m β} [Finite α m] (it : Iter (α := α) m β) : m (List β) :=
   Array.toList <$> it.toArray
 
 @[specialize]
 def Iter.drain {α : Type u} {m : Type w → Type w'} {β : Type v} [Monad m]
-    {_ : Iterator α m β} [Finite α m] {_ : ComputableSmall α} (it : Iter (α := α) m β) : m PUnit := do
-  it.stepH _ (match · with
+    {_ : Iterator α m β} [Finite α m] (it : Iter (α := α) m β) : m PUnit := do
+  match (← it.stepH).inflate with
   | .yield it' _ _ => it'.drain
   | .skip it' _ => it'.drain
-  | .done _ => return ⟨⟩)
+  | .done _ => return ⟨⟩
 termination_by it.terminationByFinite
