Iterator/Producers.lean
@@ -10,7 +10,7 @@ import Init.Data.Nat.Lemmas
 
 section ListIterator
 
-variable {m : Type w → Type w'}
+variable {α : Type u} {m : Type w → Type w'}
 
 structure ListIterator (α : Type u) where
   list : List α
@@ -41,42 +41,33 @@ structure ListIterator (α : Type u) where
 --     cases it
 --     split at h <;> simp_all [IterStep.successor]
 
-instance {α} : Iterator (ListIterator α) m α where
-  step it :=
-    { property
-        | .yield it' out => it.list = out :: it'.list
-        | .skip _ => False
-        | .done => it.list = []
-      computation := pure (match it.list with
-        | [] => ⟨.done, rfl⟩
-        | x :: xs => ⟨.yield ⟨xs⟩ x, rfl⟩) }
-    -- (fun
-    --   | [] => .done
-    --   | x :: xs => .yield { list := xs } x) <$>
-    -- (pure it.list : IterationT m _)
+instance {α : Type u} [Pure m] [UnivLE.{u, w}] : Iterator (ListIterator α) m α where
+  state_small := inferInstance
+  value_small := inferInstance
+  plausible_step it
+    | .yield it' out => it.list = out :: it'.list
+    | .skip _ => False
+    | .done => it.list = []
+  step it := pure (match it with
+        | ⟨[]⟩ => .deflate ⟨.done, rfl⟩
+        | ⟨x :: xs⟩ => .deflate ⟨.yield ⟨xs⟩ x, rfl⟩)
 
 /--
 Returns a finite iterator for the given list.
 The iterator yields the elements of the list in order and then terminates.
 -/
 @[always_inline, inline]
-def List.iter {α : Type u} (l : List α) (m : Type u → Type w := by exact Id) [ComputableSmall.{w} α] :
+def List.iter {α : Type u} (l : List α) (m : Type u → Type w := by exact Id) [Pure m] :
     Iter (α := ListIterator α) m α :=
   toIter m { list := l }
 
-instance : FinitenessRelation (ListIterator α) m where
+instance [Pure m] [UnivLE.{u, w}] : FinitenessRelation (ListIterator α) m where
   rel := InvImage WellFoundedRelation.rel ListIterator.list
   wf := InvImage.wf _ WellFoundedRelation.wf
   subrelation {it it'} h := by
     simp_wf
-    simp only [Iterator.step, IterationT.map_eq_mapH, IterationT.mapH, Pure.pure] at h
     obtain ⟨step, h, h'⟩ := h
-    cases step <;> simp_all [IterStep.successor]
-
--- TODO
--- @[inline]
--- def List.iterH {α : Type u} (l : List α) (m) [Pure m] : Iter (α := ListIterator α) m α :=
---   toIter m { list := l }
+    cases step <;> simp_all [IterStep.successor, Iterator.plausible_step]
 
 end ListIterator
 
@@ -89,18 +80,24 @@ variable {α : Type u} {m : Type w → Type w'} {f : α → α}
 structure UnfoldIterator (α : Type u) (f : α → α) where
   next : α
 
-instance : Iterator (UnfoldIterator α f) m α where
-  step it := pure <| .yield ⟨f it.next⟩ it.next
+instance [Pure m] [UnivLE.{u, w}] : Iterator (UnfoldIterator α f) m α where
+  state_small := inferInstance
+  value_small := inferInstance
+  plausible_step it
+    | .yield it' out => out = it.next ∧ it' = ⟨f it.next⟩
+    | .skip _ => False
+    | .done => False
+  step it := pure <| .deflate <| .yield ⟨f it.next⟩ it.next (by simp)
 
 /--
 Creates an infinite, productive iterator. First it yields `init`.
 If the last step yielded `a`, the next will yield `f a`.
 -/
 @[inline]
-def Iter.unfold (m : Type w → Type w' := by exact Id) {α : Type u} (init : α) (f : α → α) [ComputableUnivLE.{u, w}] :=
+def Iter.unfold (m : Type u → Type w') [Pure m] {α : Type u} (init : α) (f : α → α) :=
   toIter m <| UnfoldIterator.mk (f := f) init
 
-instance [Pure m] : ProductivenessRelation (UnfoldIterator α f) m where
+instance [Pure m] [UnivLE.{u, w}] : ProductivenessRelation (UnfoldIterator α f) m where
   rel := emptyWf.rel
   wf := emptyWf.wf
   subrelation {it it'} h := by cases h
