Iterator/UnivLE.lean
@@ -6,93 +6,147 @@ Authors: Paul Reichert
 prelude
 import Init.Core
 import Init.SimpLemmas
-
-class ComputableUnivLE.{u, v} where
-  Lift : Type u → Type v
-  up : ∀ {α}, α → Lift α
-  down : ∀ {α}, Lift α → α
-  up_down : ∀ {α : Type u} {a : Lift α}, up (down a) = a
-  down_up : ∀ {α : Type u} {a : α}, down (up a) = a
-
-instance ComputableUnivLE.self : ComputableUnivLE.{u, u} where
-  Lift α := α
-  up := id
-  down := id
-  up_down := rfl
-  down_up := rfl
-
-instance ComputableUnivLE.ofMax [i : ComputableUnivLE.{max u v, v}] : ComputableUnivLE.{u, v} where
-  Lift α := i.Lift (ULift α)
-  up x := i.up (ULift.up x)
-  down x := ULift.down (i.down x)
-  up_down {_ _} := by
-    simp only [ULift.up_down]
-    rw [ComputableUnivLE.up_down]
-  down_up := by
-    simp [ULift.down_up, ComputableUnivLE.down_up]
-
-instance ComputableUnivLE.zero : ComputableUnivLE.{0, u} := inferInstance
-
-def ComputableUnivLE.trans.{v} [iuv : ComputableUnivLE.{u, v}] [ivw : ComputableUnivLE.{v, w}] : ComputableUnivLE.{u, w} where
-  Lift α := α |> iuv.Lift |> ivw.Lift
-  up x := x |> iuv.up |> ivw.up
-  down x := x |> ivw.down |> iuv.down
-  up_down := by simp [ComputableUnivLE.up_down]
-  down_up := by simp [ComputableUnivLE.down_up]
-
-class ComputableSmall.{v, u} (α : Type u) where
-  Lift : Type v
-  up : α → Lift
-  down : Lift → α
-  up_down : ∀ {a}, up (down a) = a
-  down_up : ∀ {a}, down (up a) = a
-
-@[always_inline, inline]
-def ComputableSmall.Lift.down {α : Type u} [ComputableSmall α] : ComputableSmall.Lift α → α :=
-  ComputableSmall.down
-
-instance [ComputableUnivLE.{u, v}] {α} : ComputableSmall.{v, u} α where
-  Lift := ComputableUnivLE.Lift α
-  up := ComputableUnivLE.up
-  down := ComputableUnivLE.down
-  up_down := ComputableUnivLE.up_down
-  down_up := ComputableUnivLE.down_up
-
-@[always_inline, inline]
-def ComputableSmall.equiv [ComputableSmall.{v} α] (f : α → β) (g : β → α)
-    (hfg : ∀ {a}, f (g a) = a) (hgf : ∀ {a}, g (f a) = a) : ComputableSmall.{v} β where
-  Lift := ComputableSmall.Lift (α := α)
-  up x := ComputableSmall.up (g x)
-  down x := f (ComputableSmall.down x)
-  up_down := by simp [hgf, ComputableSmall.up_down]
-  down_up := by simp [hfg, ComputableSmall.down_up]
-
-section Tests
+import Init.NotationExtra
+import Init.Classical
 
 universe u v
 
-#guard_msgs in
-example := inferInstanceAs ComputableUnivLE.{0, u}
+class ComputableSmall (α : Type v) where
+  Target : Type u
+  deflate : α → Target
+  inflate : Target → α
+  deflate_inflate : ∀ {a}, deflate (inflate a) = a
+  inflate_deflate : ∀ {a}, inflate (deflate a) = a
+
+class Small (α : Type v) : Prop where
+  h : Nonempty (ComputableSmall.{u} α)
+
+noncomputable def ComputableSmall.choose (α : Type v) [small : Small.{u} α] : ComputableSmall.{u} α :=
+  haveI : Nonempty (ComputableSmall.{u} α) := Small.h
+  Classical.ofNonempty (α := ComputableSmall.{u} α)
+
+variable {α : Type v} {β : Type u}
+
+structure USquash (α : Type v) [small : Small.{u} α] where
+  mk' ::
+  inner : (ComputableSmall.choose α).Target
+
+private unsafe def USquash.unsafeDeflate [Small.{u} α] : α → USquash.{u} α := unsafeCast
+private unsafe def USquash.unsafeInflate [Small.{u} α] : USquash.{u} α → α := unsafeCast
+
+@[implemented_by USquash.unsafeDeflate]
+noncomputable def USquash.deflate [small : Small.{u} α] (x : α) : USquash.{u} α := USquash.mk' (ComputableSmall.choose α |>.deflate x)
+
+@[implemented_by USquash.unsafeInflate]
+noncomputable def USquash.inflate [small : Small.{u} α] (x : USquash.{u} α) : α := ComputableSmall.choose α |>.inflate x.inner
+
+@[simp]
+theorem USquash.deflate_inflate {_ : Small.{u} α} {x : USquash.{u} α} :
+    USquash.deflate x.inflate = x := by
+  simp [deflate, inflate, ComputableSmall.deflate_inflate]
+
+@[simp]
+theorem USquash.inflate_deflate {_ : Small.{u} α} {x : α} :
+    (USquash.deflate.{u} x).inflate = x := by
+  simp [deflate, inflate, ComputableSmall.inflate_deflate]
+
+attribute [deprecated "never use!" (since := "2025-04-28")]
+  USquash.inner USquash.mk'
+
+class UnivLE where
+  small : ∀ α : Type u, Small.{v} α
+
+instance [UnivLE.{u, v}] {α : Type u} : Small.{v} α := UnivLE.small α
+
+instance UnivLE.self : UnivLE.{u, u} where
+  small α := ⟨⟨{
+    Target := α
+    deflate := id
+    inflate := id
+    deflate_inflate := rfl
+    inflate_deflate := rfl }⟩⟩
+
+set_option pp.universes true in
+instance UnivLE.ofMax [i : UnivLE.{max u v, v}] : UnivLE.{u, v} where
+  small α := ⟨⟨{
+    Target := ComputableSmall.choose.{v} (ULift.{v} α) |>.Target
+    deflate x := ComputableSmall.choose.{v} (ULift.{v} α) |>.deflate (ULift.up x)
+    inflate x := ULift.down (ComputableSmall.choose.{v} (ULift.{v} α) |>.inflate x)
+    deflate_inflate {_} := by simp [ULift.up_down, ComputableSmall.deflate_inflate]
+    inflate_deflate {_} := by simp [ULift.down_up, ComputableSmall.inflate_deflate]
+  }⟩⟩
+
+instance UnivLE.zero : UnivLE.{0, u} := inferInstance
+
+def ComputableUnivLE.trans [iuv : UnivLE.{u, v}] [ivw : UnivLE.{v, w}] : UnivLE.{u, w} where
+  small α := ⟨⟨{
+    Target := α |> (ComputableSmall.choose.{v} · |>.Target) |> (ComputableSmall.choose.{w} · |>.Target)
+    deflate x := x |> (ComputableSmall.choose.{v} _).deflate |> (ComputableSmall.choose.{w} _).deflate
+    inflate x := x |> (ComputableSmall.choose.{w} _).inflate |> (ComputableSmall.choose.{v} _).inflate
+    deflate_inflate := by simp [ComputableSmall.deflate_inflate]
+    inflate_deflate := by simp [ComputableSmall.inflate_deflate]
+  }⟩⟩
+
+instance {α : Type v} [Small.{u} α] {p : α → Prop} : Small.{u} (Subtype p) where
+  h := ⟨{
+    Target := Subtype (p ∘ USquash.inflate : USquash.{u} α → Prop)
+    deflate x := ⟨USquash.deflate x.1, by simp [x.2]⟩
+    inflate x := ⟨USquash.inflate x.1, x.2⟩
+    deflate_inflate := by simp
+    inflate_deflate := by simp }⟩
+
+instance {α : Type v} [Small.{u} α] : Small.{u} (Option α) where
+  h := ⟨{
+    Target := Option (USquash α)
+    deflate x := x.map .deflate
+    inflate x := x.map USquash.inflate
+    deflate_inflate {x} := by cases x <;> simp
+    inflate_deflate {x} := by cases x <;> simp }⟩
+
+-- @[always_inline, inline]
+-- def ComputableSmall.Target.down {α : Type u} [ComputableSmall α] : ComputableSmall.Lift α → α :=
+--   ComputableSmall.down
+
+-- instance [ComputableUnivLE.{u, v}] {α} : ComputableSmall.{v, u} α where
+--   Lift := ComputableUnivLE.Lift α
+--   up := ComputableUnivLE.up
+--   down := ComputableUnivLE.down
+--   up_down := ComputableUnivLE.up_down
+--   down_up := ComputableUnivLE.down_up
+
+-- @[always_inline, inline]
+-- def ComputableSmall.equiv [ComputableSmall.{v} α] (f : α → β) (g : β → α)
+--     (hfg : ∀ {a}, f (g a) = a) (hgf : ∀ {a}, g (f a) = a) : ComputableSmall.{v} β where
+--   Lift := ComputableSmall.Lift (α := α)
+--   up x := ComputableSmall.up (g x)
+--   down x := f (ComputableSmall.down x)
+--   up_down := by simp [hgf, ComputableSmall.up_down]
+--   down_up := by simp [hfg, ComputableSmall.down_up]
+
+section Tests
 
 #guard_msgs in
-example := inferInstanceAs ComputableUnivLE.{0, 1}
+example := inferInstanceAs UnivLE.{0, u}
 
 #guard_msgs in
-example := inferInstanceAs ComputableUnivLE.{1, u + 1}
+example := inferInstanceAs UnivLE.{0, 1}
 
 #guard_msgs in
-example := inferInstanceAs ComputableUnivLE.{u, max u v}
+example := inferInstanceAs UnivLE.{1, u + 1}
 
 #guard_msgs in
-example := inferInstanceAs ComputableUnivLE.{u + 1, max u v + 1}
+example := inferInstanceAs UnivLE.{u, max u v}
+
+#guard_msgs in
+example := inferInstanceAs UnivLE.{u + 1, max u v + 1}
 
 /--
 error: failed to synthesize
-  ComputableUnivLE
+  UnivLE
 
 Additional diagnostic information may be available using the `set_option diagnostics true` command.
 -/
 #guard_msgs in
-example [ComputableUnivLE.{u, v}] [ComputableUnivLE.{u', v}] := inferInstanceAs ComputableUnivLE.{max u u', v}
+example [UnivLE.{u, v}] [UnivLE.{u', v}] := inferInstanceAs UnivLE.{max u u', v}
 
 end Tests
