Iterator/Wrapper.lean
@@ -11,99 +11,88 @@ import Iterator.Cont
 variable {α : Type u} {m : Type w → Type w'} {β : Type v}
 
 structure Iter {α : Type u} (m : Type w → Type w') (β : Type v)
-    [Iterator α m β] [small : ComputableSmall.{w} α] : Type w where
-  innerLifted : ComputableSmall.Lift α
+    [i : Iterator α m β] : Type w where
+  innerLifted : USquash.{w} (small := i.state_small) α
 
 variable (m) in
 @[always_inline, inline]
-def toIter [Iterator α m β] [ComputableSmall.{w} α] (it : α) : Iter (α := α) m β :=
-  ⟨ComputableSmall.up it⟩
+def toIter [Iterator α m β] (it : α) : Iter (α := α) m β :=
+  ⟨USquash.deflate (small := _) it⟩
 
 @[always_inline, inline]
-def Iter.inner {_ : Iterator α m β} {_ : ComputableSmall.{w} α} (it : Iter (α := α) m β) : α :=
-  ComputableSmall.down it.innerLifted
+def Iter.inner {_ : Iterator α m β} (it : Iter (α := α) m β) : α :=
+  USquash.inflate (small := _) it.innerLifted
 
 @[simp]
-theorem inner_toIter {_ : Iterator α m β} {_ : ComputableSmall.{w} α} (it : α) :
+theorem inner_toIter {_ : Iterator α m β} (it : α) :
     (toIter m it).inner = it :=
-  ComputableSmall.down_up
+  USquash.inflate_deflate
 
-def Iterator.stepLift [Iterator α m β] [ComputableSmall.{w} α] [ComputableSmall.{w} β] (it : α) :
-    IterationT m (IterStep (ComputableSmall.Lift α) (ComputableSmall.Lift β)) :=
-  Iterator.step (m := m) it |>.mapH (·.map ComputableSmall.up ComputableSmall.up)
-
-def Iterator.stepLiftState [Iterator α m β] [ComputableSmall.{w} α] (it : α) :
-    IterationT m (IterStep (ComputableSmall.Lift α) β) :=
-  Iterator.step (m := m) it |>.mapH (·.map ComputableSmall.up id)
-
-def Iter.plausible_step {_ : Iterator α m β} {_ : ComputableSmall.{w} α} (it : Iter (α := α) m β)
+def Iter.plausible_step {_ : Iterator α m β} (it : Iter (α := α) m β)
     (step : IterStep (Iter (α := α) m β) β) : Prop :=
-  Iterator.step (m := m) it.inner |>.mapH (·.map (toIter m) id) |>.property step
+  Iterator.plausible_step m it.inner (step.map Iter.inner id)
 
-def Iter.Step {_ : Iterator α m β} {_ : ComputableSmall.{w} α} (it : Iter (α := α) m β) :=
+def Iter.Step {_ : Iterator α m β} (it : Iter (α := α) m β) :=
   { step : IterStep (Iter (α := α) m β) β // it.plausible_step step }
-  -- Iterator.step (m := m) it.inner |>.mapH (·.map (toIter m) id) |>.Plausible
-
-def Iter.Step.toPlausible {_ : Iterator α m β} {_ : ComputableSmall.{w} α} {it : Iter (α := α) m β}
-    (step : Iter.Step it) :
-    Iterator.step (m := m) it.inner |>.mapH (·.map (toIter m) id) |>.Plausible :=
-  step
 
 @[match_pattern]
-def Iter.Step.yield {_ : Iterator α m β} {_ : ComputableSmall.{w} α}
-   {it : Iter (α := α) m β} (it' b h) := (⟨.yield it' b, h⟩ : it.Step)
+def Iter.Step.yield {_ : Iterator α m β} {it : Iter (α := α) m β} (it' b h) :=
+  (⟨.yield it' b, h⟩ : it.Step)
 
 @[match_pattern]
-def Iter.Step.skip {_ : Iterator α m β} {_ : ComputableSmall.{w} α}
-   {it : Iter (α := α) m β} (it' h) := (⟨.skip it', h⟩ : it.Step)
+def Iter.Step.skip {_ : Iterator α m β} {it : Iter (α := α) m β} (it' h) :=
+  (⟨.skip it', h⟩ : it.Step)
 
 @[match_pattern]
-def Iter.Step.done {_ : Iterator α m β} {_ : ComputableSmall.{w} α}
-   {it : Iter (α := α) m β} (h) := (⟨.done, h⟩ : it.Step)
+def Iter.Step.done {_ : Iterator α m β} {it : Iter (α := α) m β} (h) :=
+  (⟨.done, h⟩ : it.Step)
 
--- inductive Iter.Step {_ : Iterator α m β} {_ : ComputableSmall.{w} α} (it : Iter (α := α) m β) where
--- | yield : (it' : Iter (α := α) m β) → (b : β) → Iterator.yielded m it.inner it'.inner b → it.Step
--- | skip : (it' : Iter (α := α) m β) → Iterator.skipped m it.inner it'.inner → it.Step
--- | done : Iterator.done m it.inner → it.Step
+instance {_ : Iterator α m β} :
+    Small.{w} (IterStep (Iter (α := α) m β) β) :=
+  haveI : Small.{w} β := Iterator.value_small α m
+  inferInstance
 
-def Iter.LiftedStep {_ : Iterator α m β} {_ : ComputableSmall.{w} α} [ComputableSmall.{w} β]
-   (it : Iter (α := α) m β) : Type w :=
-  Iterator.step (m := m) it.inner |>.mapH (·.map (fun x => toIter m x) ComputableSmall.up) |>.Plausible
+instance {_ : Iterator α m β} {it : Iter (α := α) m β} :
+    Small.{w} it.Step where
+  h := ⟨{
+    Target := { step : USquash.{w} (IterStep (Iter (α := α) m β) β) // it.plausible_step step.inflate }
+    deflate x := ⟨.deflate (small := _) x.1, by simp [x.2]⟩
+    inflate x := ⟨x.1.inflate, x.2⟩
+    deflate_inflate := by simp
+    inflate_deflate {x} := by cases x; simp
+  }⟩
+
+set_option pp.universes true in
+def Iter.LiftedStep {_ : Iterator α m β} (it : Iter (α := α) m β) : Type w :=
+  { step : IterStep (Iter (α := α) m β) (USquash.{w} (small := Iterator.value_small α m)) //
+    it.plausible_step (step.map id (USquash.inflate (small := _))) }
 
 @[match_pattern]
-def Iter.LiftedStep.yield {_ : Iterator α m β} {_ : ComputableSmall.{w} α} [ComputableSmall.{w} β]
+def Iter.LiftedStep.yield {_ : Iterator α m β}
    {it : Iter (α := α) m β} (it' b h) := (⟨.yield it' b, h⟩ : it.LiftedStep)
 
 @[match_pattern]
-def Iter.LiftedStep.skip {_ : Iterator α m β} {_ : ComputableSmall.{w} α} [ComputableSmall.{w} β]
+def Iter.LiftedStep.skip {_ : Iterator α m β}
    {it : Iter (α := α) m β} (it' h) := (⟨.skip it', h⟩ : it.LiftedStep)
 
 @[match_pattern]
-def Iter.LiftedStep.done {_ : Iterator α m β} {_ : ComputableSmall.{w} α} [ComputableSmall.{w} β]
+def Iter.LiftedStep.done {_ : Iterator α m β}
    {it : Iter (α := α) m β} (h) := (⟨.done, h⟩ : it.LiftedStep)
 
--- inductive Iter.LiftedStep {_ : Iterator α m β} {_ : ComputableSmall.{w} α} [ComputableSmall.{w} β]
---     (it : Iter (α := α) m β) where
--- | yield : (it' : Iter (α := α) m β) → (b : ComputableSmall.Lift.{w} β) → Iterator.yielded m it.inner it'.inner (ComputableSmall.down b) → it.LiftedStep
--- | skip : (it' : Iter (α := α) m β) → Iterator.skipped m it.inner it'.inner → it.LiftedStep
--- | done : Iterator.done m it.inner → it.LiftedStep
+@[always_inline, inline]
+def Iter.Step.lift {_ : Iterator α m β} (it : Iter (α := α) m β) (step : it.Step) : it.LiftedStep :=
+  ⟨step.val.map id (USquash.deflate (small := _)),
+   by simp [IterStep.map_map, IterStep.map_id', step.property]⟩
 
 @[always_inline, inline]
-def Iter.Step.lift {_ : Iterator α m β} {_ : ComputableSmall.{w} α} [ComputableSmall.{w} β]
-    (it : Iter (α := α) m β) (step : it.Step) : it.LiftedStep := by
-  refine step.toPlausible.map (fun s => s.map id ComputableSmall.up) |>.copy ?_
-  simp [Iterator.stepLift, Iterator.stepLiftState, IterationT.mapH_mapH, IterStep.map_map]
+def Iter.Step.ofInternal {_ : Iterator α m β} (it : Iter (α := α) m β) (step : PlausibleIterStep (Iterator.plausible_step m it.inner)) :
+    it.Step :=
+  ⟨step.1.map (toIter m) id, by simp [Iter.plausible_step, IterStep.map_map, IterStep.map_id', step.2]⟩
 
 @[always_inline, inline]
-def Iter.Step.ofInternal {_ : Iterator α m β} {_ : ComputableSmall.{w} α} (it : Iter (α := α) m β) (step : Iterator.step (m := m) it.inner |>.Plausible) :
-    it.Step := by
-  exact step.map _
-
-@[always_inline, inline]
-def Iter.Step.toInternal {_ : Iterator α m β} {_ : ComputableSmall.{w} α} (it : Iter (α := α) m β) (step : it.Step) :
-    Iterator.step (m := m) it.inner |>.Plausible := by
-  refine step.toPlausible.map (fun s => s.map Iter.inner id) |>.copy ?_
-  simp only [IterationT.mapH_mapH, inner_toIter, IterStep.map_map, id_eq, IterStep.map_id', IterationT.mapH_id']
+def Iter.Step.toInternal {_ : Iterator α m β} (it : Iter (α := α) m β) (step : it.Step) :
+    PlausibleIterStep (Iterator.plausible_step m it.inner) :=
+  ⟨step.1.map Iter.inner id, step.2⟩
 
 -- instance {m} [Functor m] [Iterator α m β] : Iterator (Iter (α := α) m β) m β where
 --   yielded it it' b := Iterator.yielded m it.inner it'.inner b
@@ -122,14 +111,14 @@ def Iter.Step.toInternal {_ : Iterator α m β} {_ : ComputableSmall.{w} α} (it
 --   wf := InvImage.wf (productiveIteratorWF ∘ Iter.inner ∘ ProductiveIteratorWF.inner) Productive.wf
 
 @[always_inline, inline]
-def Iter.stepH [Monad m] {_ : Iterator α m β} {_ : ComputableSmall.{w} α} (it : Iter (α := α) m β) :
-    CodensityT m it.Step :=
-  Iterator.step it.inner |>.computation |>.mapH (Iter.Step.ofInternal it)
+def Iter.stepH [Monad m] {_ : Iterator α m β} (it : Iter (α := α) m β) :
+    m (USquash it.Step) :=
+  (fun x => Iter.Step.ofInternal it (x.inflate (small := _)) |> .deflate) <$> Iterator.step (m := m) it.inner
 
 @[always_inline, inline]
-def Iter.step {β : Type w} [Monad m] {_ : Iterator α m β} {_ : ComputableSmall.{w} α} (it : Iter (α := α) m β) :
+def Iter.step {β : Type w} [Monad m] {_ : Iterator α m β} (it : Iter (α := α) m β) :
     m (Iter.Step it) :=
-  it.stepH.run
+  USquash.inflate <$> it.stepH
 
 section Finite
 
@@ -137,12 +126,12 @@ structure Iter.FiniteWFRel (α : Type u) (m : Type w → Type w') [Iterator α m
   inner : α
 
 @[always_inline, inline]
-def Iter.terminationByFinite {_ : Iterator α m β} {_ : ComputableSmall.{w} α} [Finite α m] (it : Iter (α := α) m β) :
+def Iter.terminationByFinite {_ : Iterator α m β} [Finite α m] (it : Iter (α := α) m β) :
     Iter.FiniteWFRel α m :=
   ⟨it.inner⟩
 
 def Iter.FiniteWFRel.rel [Iterator α m β] [Finite α m] : FiniteWFRel α m → FiniteWFRel α m → Prop :=
-  InvImage (Iterator.successor_of m) Iter.FiniteWFRel.inner
+  InvImage (Iterator.plausible_successor m) Iter.FiniteWFRel.inner
 
 instance [Iterator α m β] [Finite α m] : WellFoundedRelation (Iter.FiniteWFRel α m) where
   rel := Iter.FiniteWFRel.rel
@@ -157,48 +146,41 @@ private theorem Option.elim_id {α : Type u} (o : Option α) :
     o.elim none (some ·) = o := by
   cases o <;> rfl
 
-def Iter.FiniteWFRel.of_step_yield {α m β} {_ : Iterator α m β} [Finite α m] {_ : ComputableSmall.{w} α}
-    {it' it : Iter (α := α) m β} {out : β} (h : (Iterator.step (m := m) it.inner).mapH (·.map (toIter m) id) |>.property (.yield it' out)) : Iter.FiniteWFRel.rel it'.terminationByFinite it.terminationByFinite := by
-  simp_wf
-  simp [Iter.FiniteWFRel.rel, Iterator.successor_of]
-  refine ⟨.yield it'.inner out, rfl, ?_⟩
-  have h' : (Iterator.step (m := m) it.inner).mapH (·.map (toIter m) id) |>.mapH (·.map Iter.inner id) |>.property (.yield it'.inner out) :=
-    ⟨_, rfl, h⟩
-  simpa only [IterationT.mapH_mapH, IterStep.map_map, inner_toIter, id_eq, IterStep.map_id', IterationT.mapH_id'] using h'
-
-def Iter.FiniteWFRel.of_step_skip {α m β} {_ : Iterator α m β} [Finite α m] {_ : ComputableSmall.{w} α}
-    {it' it : Iter (α := α) m β} (h : (Iterator.step (m := m) it.inner).mapH (·.map (toIter m) id) |>.property (.skip it')) : Iter.FiniteWFRel.rel it'.terminationByFinite it.terminationByFinite := by
-  simp_wf
-  simp [Iter.FiniteWFRel.rel, Iterator.successor_of]
-  refine ⟨.skip it'.inner, rfl, ?_⟩
-  have h' : (Iterator.step (m := m) it.inner).mapH (·.map (toIter m) id) |>.mapH (·.map Iter.inner id) |>.property (.skip it'.inner) :=
-    ⟨_, rfl, h⟩
-  simpa only [IterationT.mapH_mapH, IterStep.map_map, inner_toIter, id_eq, IterStep.map_id', IterationT.mapH_id'] using h'
-
-def Iter.FiniteWFRel.of_stepH_yield {α m β} {_ : Iterator α m β} [Finite α m]
-    {_ : ComputableSmall.{w} α} {_ : ComputableSmall.{w} β}
-    {it' it : Iter (α := α) m β} {out : ComputableSmall.Lift β}
-    (h : (Iterator.step (m := m) it.inner).mapH (·.map (toIter m) ComputableSmall.up) |>.property (.yield it' out)) :
+def Iter.FiniteWFRel.of_step_yield {α m β} {_ : Iterator α m β} [Finite α m]
+    {it' it : Iter (α := α) m β} {out : β} (h : it.plausible_step (.yield it' out)) :
     Iter.FiniteWFRel.rel it'.terminationByFinite it.terminationByFinite := by
-  apply Iter.FiniteWFRel.of_step_yield
-  simpa [IterationT.mapH_mapH, IterStep.map_map, ComputableSmall.down_up] using
-    IterationT.property_mapH (·.map id ComputableSmall.down) h
+  simp [terminationByFinite, Iter.FiniteWFRel.rel, Iterator.plausible_successor, InvImage]
+  exact ⟨.yield it'.inner out, rfl, h⟩
 
-def Iter.FiniteWFRel.of_stepH_skip {α m β} {_ : Iterator α m β} [Finite α m]
-    {_ : ComputableSmall.{w} α} {_ : ComputableSmall.{w} β}
-    {it' it : Iter (α := α) m β}
-    (h : (Iterator.step (m := m) it.inner).mapH (·.map (toIter m) ComputableSmall.up) |>.property (.skip it')) :
-    Iter.FiniteWFRel.rel it'.terminationByFinite it.terminationByFinite := by
-  apply Iter.FiniteWFRel.of_step_skip
-  simpa [IterationT.mapH_mapH, IterStep.map_map, ComputableSmall.down_up] using
-    IterationT.property_mapH (·.map id ComputableSmall.down) h
+def Iter.FiniteWFRel.of_step_skip {α m β} {_ : Iterator α m β} [Finite α m]
+    {it' it : Iter (α := α) m β} (h : it.plausible_step (.skip it')) : Iter.FiniteWFRel.rel it'.terminationByFinite it.terminationByFinite := by
+  simp [terminationByFinite, Iter.FiniteWFRel.rel, Iterator.plausible_successor, InvImage]
+  exact ⟨.skip it'.inner, rfl, h⟩
+
+-- def Iter.FiniteWFRel.of_stepH_yield {α m β} {_ : Iterator α m β} [Finite α m]
+--     {it' it : Iter (α := α) m β} {out : β}
+--     (h : it.plausible_step (.yield it' out)) :
+--     Iter.FiniteWFRel.rel it'.terminationByFinite it.terminationByFinite := by
+--   apply Iter.FiniteWFRel.of_step_yield
+--   simpa [IterationT.mapH_mapH, IterStep.map_map, ComputableSmall.down_up] using
+--     IterationT.property_mapH (·.map id ComputableSmall.down) h
+
+-- def Iter.FiniteWFRel.of_stepH_skip {α m β} {_ : Iterator α m β} [Finite α m]
+--     {_ : ComputableSmall.{w} α} {_ : ComputableSmall.{w} β}
+--     {it' it : Iter (α := α) m β}
+--     (h : (Iterator.step (m := m) it.inner).mapH (·.map (toIter m) ComputableSmall.up) |>.property (.skip it')) :
+--     Iter.FiniteWFRel.rel it'.terminationByFinite it.terminationByFinite := by
+--   apply Iter.FiniteWFRel.of_step_skip
+--   simpa [IterationT.mapH_mapH, IterStep.map_map, ComputableSmall.down_up] using
+--     IterationT.property_mapH (·.map id ComputableSmall.down) h
 
 macro_rules | `(tactic| decreasing_trivial) => `(tactic|
   first
   | exact Iter.FiniteWFRel.of_step_yield ‹_›
   | exact Iter.FiniteWFRel.of_step_skip ‹_›
-  | exact Iter.FiniteWFRel.of_stepH_yield ‹_›
-  | exact Iter.FiniteWFRel.of_stepH_skip ‹_›)
+  -- | exact Iter.FiniteWFRel.of_stepH_yield ‹_›
+  -- | exact Iter.FiniteWFRel.of_stepH_skip ‹_›
+  )
 
 end Finite
 
